model a part of simpl1

coq/Mini.v
@@ -7,6 +7,7 @@ Inductive expr :=
 | Or (l : list expr)
 | Imply (a b : expr)
 | Not (a : expr)
+| ETrue | EFalse
 | Unknown (R : Rest) (l : list expr)
 | UnknownAtom (R : Rest).
 
@@ -25,6 +26,8 @@ Fixpoint BDenote (e : expr) : bool :=
   | Or l => existsb BDenote l
   | Imply a b => implb (BDenote a) (BDenote b)
   | Not a => negb (BDenote a)
+  | ETrue => true
+  | EFalse => false
   | Unknown R l => UnknownDenote R l
   | UnknownAtom R => UnknownAtomDenote R
   end.
@@ -37,6 +40,8 @@ Fixpoint Size (e : expr) :=
     | Or l => (fold_left plus (map Size l) 0)
     | Imply a b => (Size a + Size b)
     | Not a => Size a
+    | ETrue => 0
+    | EFalse => 0
     | Unknown R l => (fold_left plus (map Size l) 0)
     | UnknownAtom R => 0
     end.
@@ -68,6 +73,8 @@ Fixpoint IfAnd (ex : expr) : expr :=
   | Or l => Or (map IfAnd l)
   | Imply l r => Imply (IfAnd l) (IfAnd r)
   | Not a => Not (IfAnd a)
+  | ETrue => ETrue
+  | EFalse => EFalse
   | Unknown r l => Unknown r (map IfAnd l)
   | UnknownAtom r => UnknownAtom r
   end.
@@ -82,15 +89,18 @@ Program Fixpoint expr_ind_Forall
   (POr : forall l, Forall P l -> P (Or l))
   (PImply : forall a b, P a -> P b -> P (Imply a b))
   (PNot : forall a, P a -> P (Not a))
+  (PETrue : P ETrue) (PEFalse : P EFalse)
   (PUnknown : forall R l, Forall P l -> P (Unknown R l))
   (PUnknownAtom : forall R, P (UnknownAtom R)) e : P e :=
-  let F := (expr_ind_Forall P PIf PAnd POr PImply PNot PUnknown PUnknownAtom) in
+  let F := (expr_ind_Forall P PIf PAnd POr PImply PNot PETrue PEFalse PUnknown PUnknownAtom) in
     match e with
     | If a b c => PIf a b c (F a) (F b) (F c)
     | And l => PAnd l (list_ind _ _ (fun ex _ _ => Forall_cons ex (F ex) _) l)
     | Or l => POr l (list_ind _ _ (fun ex _ _ => Forall_cons ex (F ex) _) l)
     | Imply a b => PImply a b (F a) (F b)
     | Not a => PNot a (F a)
+    | ETrue => PETrue
+    | EFalse => PEFalse
     | Unknown R l => PUnknown R l (list_ind _ _ (fun ex _ _ => Forall_cons ex (F ex) _) l)
     | UnknownAtom R => PUnknownAtom R
     end.
@@ -105,4 +115,39 @@ Definition IfAndPreserve : forall e, BDenote (IfAnd e) = BDenote e.
     try rewrite !IfAndRPreserve in *; try congruence).
   apply RestBDenoteModular; simpl; rewrite H2; f_equal.
   rewrite map_map; apply map_ext_in; intros; eapply Forall_forall in H3; eauto.
+Qed.
+
+Definition Simpl1 e :=
+  match e with
+  | If ETrue a _ => a
+  | If EFalse _ a => a
+  | If a ETrue EFalse => a
+  | If a EFalse ETrue => Not a
+  | If _ a b => if exprEqDec a b then a else e
+  | Imply EFalse _ => ETrue
+  | Imply ETrue a => a
+  | Not (Not a) => a
+  | And [] => ETrue
+  | And l => 
+      if In_dec exprEqDec EFalse l 
+      then EFalse 
+      else
+        let l := (remove exprEqDec ETrue l) in 
+          match l with [] => ETrue | _ => And l end
+  | Or [] => EFalse
+  | Or l => 
+      if In_dec exprEqDec ETrue l 
+      then ETrue 
+      else 
+        let l := (remove exprEqDec EFalse l) in 
+          match l with [] => EFalse | _ => Or l end
+  | _ => e
+  end.
+
+Theorem Simpl1Preserve e : BDenote (Simpl1 e) = BDenote e.
+  destruct e; simpl; try induction l;
+  repeat (
+    unfold negb in *; unfold andb in *; unfold orb in *;
+    try match goal with H : _ :: _ = _ :: _ |- _ => invcs H end;
+    try match_destruct; subst; simpl in *; try congruence).
 Qed.
